Bump Coq 8.19 and slight refactoring

fairneris/examples/retransmit_model.v
@@ -2,6 +2,7 @@ From trillium.prelude Require Export finitary quantifiers sigma classical_instan
 From Paco Require Import paco1 paco2 pacotac.
 From fairneris Require Export trace_utils fairness.
 From fairneris.aneris_lang Require Import ast network.
+From fairneris Require Export trace_utils ltl_lite.
 
 Import derived_laws_later.bi.
 
@@ -27,10 +28,6 @@ Proof. intros ??. apply make_decision. Qed.
 Proof. exact (populate (Start,∅,∅)). Qed.
 
 Inductive retransmit_node_role := Arole | Brole.
-(* Inductive retransmit_network_role := *)
-(* | Ndup *)
-(* | Ndrop *)
-(* | Ndeliver. *)
 Definition retransmit_network_role : Set := unit.
 Definition retransmit_role : Set :=
   retransmit_node_role + retransmit_network_role.
@@ -130,350 +127,392 @@ Inductive retransmit_trans : retransmit_state → retransmit_label → retransmi
                    (inl $ (Brole, None))
                    (Received, ms, <[saB := ms']>bs).
 
-Definition send_filter msg : retransmit_state → retransmit_label → Prop :=
-  λ _ l, label_action l = inl $ Some msg.
-Instance send_filter_decision msg st l : Decision (send_filter msg st l).
-Proof. apply make_decision. Qed.
-
-Definition deliver_filter msg : retransmit_state → retransmit_label → Prop :=
-  λ _ l, l = inr ((),Some msg).
-Instance deliver_filter_decision msg st l : Decision (deliver_filter msg st l).
-Proof. apply make_decision. Qed.
-
-Class Monotone (f : nat → nat) :=
-  { mono_incr : ∀ n m, n ≤ m → f n ≤ f m; }.
-
-Definition count_sends (msg : message) tr : nat :=
-  count_labels (trace_filter (send_filter msg) tr).
-
-Definition count_delivers (msg : message) tr : nat :=
-  count_labels (trace_filter (deliver_filter msg) tr).
-
 Notation mtrace := (trace retransmit_state retransmit_label).
 
-Definition retransmit_network_fair_delivery (tr : mtrace) : Prop :=
-  ∃ (f1 f2 : nat → nat) `(Monotone f1) `(Monotone f2),
-    ∀ msg n,
-      let sends := count_sends msg (trace_take n tr) in
-      let delivers := count_delivers msg (trace_take n tr) in
-      f1 delivers ≤ sends ≤ f2 delivers.
-
-(* TODO: This computation is a bit odd *)
-(* Definition retransmit_live_roles (s : retransmit_state) : gset retransmit_role := *)
-(*   {[inl Arole]} ∪ *)
-(*   (if decide (s.1.2 = (∅:gmultiset _)) then ∅ *)
-(*    else {[inr Ndup;inr Ndrop;inr Ndeliver]}) ∪ *)
-(*   (match s.1.1 with Start => {[inl Brole]} | _ => ∅ end). *)
 Definition retransmit_live_roles (s : retransmit_state) : gset retransmit_node_role :=
   {[Arole]} ∪
   (match s.1.1 with Start => {[Brole]} | _ => ∅ end).
 
-(* TODO: This should be generalised, and lifted to multiple roles *)
-Definition retransmit_terminating_role (ρ : retransmit_node_role) (tr : mtrace) : Prop :=
-  ∃ n, after n tr = None ∨
-       pred_at tr n (λ st _, ρ ∉ retransmit_live_roles st).
-
 Definition retransmit_role_enabled_model (ρ : retransmit_node_role) (s : retransmit_state) : Prop :=
   ρ ∈ retransmit_live_roles s.
-
-Definition retransmit_fair_scheduling_mtr (ρ : retransmit_node_role) : mtrace → Prop :=
-  trace_implies (λ δ _, retransmit_role_enabled_model ρ δ)
-                (λ δ ℓ, ¬ retransmit_role_enabled_model ρ δ ∨
-                          option_map label_role ℓ = Some (inl ρ)).
-
-Lemma retransmit_fair_scheduling_mtr_after ℓ tr tr' k :
-  after k tr = Some tr' →
-  retransmit_fair_scheduling_mtr ℓ tr → retransmit_fair_scheduling_mtr ℓ tr'.
-Proof. apply trace_implies_after. Qed.
-
-Definition retransmit_fair_scheduling (mtr : mtrace) : Prop :=
-  ∀ ρ, retransmit_fair_scheduling_mtr ρ mtr.
-
-Lemma retransmit_fair_scheduling_after tr tr' k :
-  after k tr = Some tr' →
-  retransmit_fair_scheduling tr → retransmit_fair_scheduling tr'.
-Proof.
-  intros Hafter Hfair ℓ. specialize (Hfair ℓ).
-  by eapply retransmit_fair_scheduling_mtr_after.
-Qed.
-
-Definition mtrace_fair (mtr : mtrace) : Prop :=
-  retransmit_fair_scheduling mtr ∧ retransmit_network_fair_delivery mtr.
-
-Inductive mtrace_valid_ind (mtrace_valid_coind: mtrace → Prop) :
-  mtrace → Prop :=
-| mtrace_valid_singleton δ: mtrace_valid_ind _ ⟨δ⟩
-| mtrace_valid_cons δ ℓ tr:
-  retransmit_trans δ ℓ (trfirst tr) →
-  mtrace_valid_coind tr →
-  mtrace_valid_ind _ (δ -[ℓ]-> tr).
-Definition mtrace_valid := paco1 mtrace_valid_ind bot1.
-
-Lemma mtrace_valid_mono :
-  monotone1 mtrace_valid_ind.
-Proof.
-  unfold monotone1. intros x0 r r' IN LE.
-  induction IN; try (econstructor; eauto; done).
-Qed.
-Hint Resolve mtrace_valid_mono : paco.
-
-Lemma mtrace_valid_after (mtr mtr' : mtrace) k :
-  after k mtr = Some mtr' → mtrace_valid mtr → mtrace_valid mtr'.
-Proof.
-  revert mtr mtr'.
-  induction k; intros mtr mtr' Hafter Hvalid.
-  { destruct mtr'; simpl in *; by simplify_eq. }
-  punfold Hvalid.
-  inversion Hvalid as [|??? Htrans Hval']; simplify_eq.
-  eapply IHk; [done|].
-  by inversion Hval'.
-Qed.
-
-Lemma retransmit_trace_delivers_0 mtr n :
-  (∀ n, pred_at mtr n (λ _ l, l ≠ Some $ inr ((), Some mAB))) →
-  count_delivers mAB (trace_take n mtr) = 0.
-Proof.
-  revert mtr.
-  induction n as [|n IHn]; intros mtr Hpred=> /=; [by destruct mtr|].
-  destruct mtr as [|s l mtr]; [done|]. rewrite /count_delivers=> /=.
-  case_bool_decide as Hb.
-  - specialize (Hpred 0). rewrite pred_at_0 in Hpred.
-    rewrite /deliver_filter in Hb. by simplify_eq.
-  - apply IHn. intros n'. specialize (Hpred (S n')).
-    by rewrite pred_at_S in Hpred.
-Qed.
-
-Lemma A_always_live (mtr : mtrace) n :
-  infinite_trace mtr →
-  pred_at mtr n (λ s _, retransmit_role_enabled_model (Arole) s).
-Proof.
-  rewrite /pred_at /retransmit_role_enabled_model. intros [mtr' ->].
-  by destruct mtr'; set_solver.
-Qed.
-
-Lemma retransmit_fair_traces_eventually_A mtr :
-  infinite_trace mtr → retransmit_fair_scheduling mtr →
-  ∃ n, pred_at mtr n (λ _ ℓ, option_map label_role ℓ = Some $ inl Arole).
-Proof.
-  intros Hinf Hfair.
-  pose proof (A_always_live mtr 0 Hinf) as HA.
-  apply Hfair in HA as [m HA]. apply pred_at_or in HA as [HA|HA]; [|by exists m].
-  pose proof (A_always_live mtr m Hinf) as HA'. by apply pred_at_neg in HA.
-Qed.
-
-Lemma retransmit_fair_traces_eventually_mAB mtr :
-  infinite_trace mtr → mtrace_valid mtr → retransmit_fair_scheduling mtr →
-  ∃ n, pred_at mtr n (λ st l, option_map label_action l = Some $ inl $ Some mAB).
-Proof.
-  intros Hinf Hvalid Hfair.
-  pose proof (retransmit_fair_traces_eventually_A mtr) as [m HA]; [done..|].
-  exists m. specialize (Hinf m) as [mtr' Hafter].
-  eapply mtrace_valid_after in Hvalid; [|done].
-  rewrite /pred_at Hafter in HA. rewrite /pred_at Hafter.
-  destruct mtr'; [done|]. destruct ℓ; [|done]. destruct r. simpl in *.
-  simplify_eq. pinversion Hvalid. inversion H1. by simplify_eq.
-Qed.
-
-(* TODO: This can possibly be generalised *)
-Lemma count_sends_pred_at n tr :
-  pred_at tr n (λ _ l, option_map label_action l = Some $ inl $ Some mAB) →
-  0 < count_sends mAB (trace_take (S n) tr).
-Proof.
-  revert tr. induction n as [|n IHn]=> /=; intros tr Hpred_at.
-  { rewrite /pred_at in Hpred_at. destruct tr; [done|].
-    rewrite /count_sends=> /=.
-    case_bool_decide as Hb; [by simpl; lia|].
-    destruct ℓ; [|done]. rewrite /send_filter in Hb.
-    destruct r. simpl in *. simplify_eq. }
-  destruct tr; [done|]. rewrite /count_sends=> /=.
-  case_bool_decide as Hb; [simpl; lia|by apply IHn].
-Qed.
-
-(* Any fair infinite trace grow the number of sends indefinitely *)
-Lemma retransmit_trace_sends_grows mtr x :
-  infinite_trace mtr → mtrace_valid mtr → retransmit_fair_scheduling mtr →
-  ∃ n, x < count_sends mAB (trace_take n mtr).
-Proof.
-  intros Hafter Hvalid Hfair.
-  induction x as [|x IHx].
-  { pose proof (retransmit_fair_traces_eventually_mAB) as [n Hn]; [done..|].
-    exists (S n). by eapply count_sends_pred_at. }
-  destruct IHx as [n Hn].
-  apply (infinite_trace_after' n) in Hafter as (mtr' & Hmtr' & Hafter).
-  apply (mtrace_valid_after _ mtr' n) in Hvalid; [|done].
-  apply (retransmit_fair_scheduling_after _ mtr' n) in Hfair; [|done].
-  pose proof (retransmit_fair_traces_eventually_mAB) as [m Hm]; [done..|].
-  assert (0 < count_sends mAB (trace_take (S m) mtr')) as Hcount.
-  { by eapply count_sends_pred_at. }
-  exists (n+(S m)).
-  rewrite /count_sends. rewrite /count_sends in Hcount.
-  rewrite /count_sends in Hn. rewrite (count_labels_sum _ _ _ _ mtr'); [lia|done].
-Qed.
-
-(* Any fair trace eventually delivers a message *)
-Lemma retransmit_fair_trace_eventually_Ndeliver mtr :
-  infinite_trace mtr → mtrace_valid mtr → mtrace_fair mtr →
-  ∃ n, pred_at mtr n (λ st l, l = Some $ inr ((),Some mAB)).
-Proof.
-  intros Hafter Hvalid Hfair.
-  assert ((∃ n, pred_at mtr n (λ _ l, l = Some (inr ((), Some mAB)))) ∨
-            ¬ ∃ n, pred_at mtr n (λ _ l, l = Some (inr ((), Some mAB))))
-    as Hpred_at.
-  { apply ExcludedMiddle. }
-  destruct Hpred_at as [Hpred_at|Hpred_at]; [done|].
-  assert False; [|done].
-  destruct Hfair as [Hfair_sched Hfair_network].
-  destruct Hfair_network as (f1&f2&?&?&Hfair_network).
-  pose proof (retransmit_trace_sends_grows mtr (f2 0)) as [m Hm]; [done..|].
-  specialize (Hfair_network mAB m).
-  destruct Hfair_network as [_ Hfair_network2].
-  rewrite retransmit_trace_delivers_0 in Hfair_network2; [lia|].
-  intros n. apply pred_at_neg; [done|].
-  by eapply not_exists_forall_not in Hpred_at.
-Qed.
-
-Lemma Ndeliver_adds_to_buffer msg s bs (mtr:mtrace) :
-  mtrace_valid (s -[inr ((),Some msg)]-> mtr) →
-  (trfirst (s -[inr ((),Some msg)]-> mtr)).2 !!! m_destination msg = bs →
-  (trfirst mtr).2 !!! (m_destination msg) = msg :: bs.
-Proof.
-  intros Hvalid <-. pinversion Hvalid; simplify_eq. inversion H1; simplify_eq.
-  by rewrite lookup_total_insert.
-Qed.
-
-Lemma retransmit_fair_trace_buffer_grows mtr n mtr' :
-  mtrace_valid mtr →
-  (∀ m, m < n → pred_at mtr m
-                  (λ _ l, option_map label_role l ≠ Some $ inl Brole)) →
-  after n mtr = Some mtr' →
-  suffix ((trfirst mtr).2 !!! saB) ((trfirst mtr').2 !!! saB).
-Proof.
-  revert mtr. induction n as [|n IHn]; intros mtr Hvalid Halways Hafter.
-  { simpl in *. by simplify_eq. }
-  destruct mtr as [|s l mtr]; [done|].
-  eapply suffix_trans; last first.
-  { apply IHn; [| |done].
-    { by eapply (mtrace_valid_after _ mtr 1); [|done]. }
-    intros m Hlt. specialize (Halways (S m)). rewrite pred_at_S in Halways.
-    apply Halways. lia. }
-  punfold Hvalid. inversion Hvalid. simplify_eq.
-  inversion H1; simplify_eq; try set_solver.
-  - destruct (decide (m_destination msg = saB)) as [->|Hneq].
-    + rewrite lookup_total_insert. apply suffix_cons_r. set_solver.
-    + by rewrite lookup_total_insert_ne.
-  - assert (0 < S n) as Hlt by lia.
-    specialize (Halways 0 Hlt). rewrite pred_at_0 in Halways. simplify_eq.
-Qed.
-
-
-(* TODO: Could use more polish. Might simplify proof as well *)
-(* Any fair trace eventually ends in the receive state *)
-Lemma retransmit_fair_trace_eventually_Received mtr :
-  (trfirst mtr).1.1 = Start →
-  infinite_trace mtr → mtrace_valid mtr → mtrace_fair mtr →
-  ∃ n, pred_at mtr n (λ st _, st.1.1 = Received).
-Proof.
-  intros Htrfirst Hafter Hvalid Hfair.
-  pose proof (retransmit_fair_trace_eventually_Ndeliver) as [n Hn]; [done..|].
-  rewrite /pred_at in Hn.
-  apply (infinite_trace_after' n) in Hafter as [mtr' [Hmtr' Hafter]].
-  destruct Hfair as [Hfair1 Hfair2].
-  assert (retransmit_fair_scheduling mtr') as Hfair1'.
-  { by eapply retransmit_fair_scheduling_after. }
-  rewrite Hmtr' in Hn. destruct mtr' as [mtr'|]; [done|].
-  simplify_eq. rewrite /retransmit_fair_scheduling in Hfair1'.
-  assert ((pred_at (s -[ inr ((), Some mAB) ]-> mtr') 0
-                   (λ δ _, retransmit_role_enabled_model (Brole) δ)) ∨
-            ¬ pred_at (s -[ inr ((), Some mAB) ]-> mtr') 0
-                   (λ δ _, retransmit_role_enabled_model (Brole) δ)) as Hrole.
-  { eapply ExcludedMiddle. }
-  destruct Hrole as [Hrole|Hrole]; last first.
-  { apply pred_at_neg in Hrole; [|done]. rewrite /pred_at in Hrole.
-    exists n. rewrite /pred_at. rewrite Hmtr'.
-    rewrite /retransmit_role_enabled_model /retransmit_live_roles in Hrole.
-    destruct s as [[[]]]; [by set_solver|done]. }
-  apply Hfair1' in Hrole as [m Hm].
-  apply pred_at_or in Hm as [Hm|Hm].
-  { exists (n+m). rewrite pred_at_sum Hmtr'. eapply pred_at_impl; [|done].
-    intros [[[]]] l Hsl; [|done].
-    rewrite /retransmit_role_enabled_model /retransmit_live_roles in Hsl.
-    set_solver. }
-  assert (∃ bs, (trfirst (s -[ inr ((), Some mAB) ]-> mtr')).2 !!!
-                  m_destination mAB = bs) as [bs Hbs].
-  { by eexists _. }
-  assert (after (S n) mtr = Some mtr') as Hmtr'2.
-  { replace (S n) with (n + 1) by lia. rewrite after_sum'. by rewrite Hmtr'. }
-  apply Ndeliver_adds_to_buffer in Hbs; [|by eapply mtrace_valid_after].
-  destruct m as [|m]; [done|]. rewrite pred_at_S in Hm.
-  pose proof (trace_eventually_until mtr') as [n' [Hn' Hn'']]; [by exists m|].
-  exists (n+(S $ S n')).
-  rewrite pred_at_sum Hmtr' pred_at_S.
-  assert (pred_at mtr' n'
-                  (λ s _, suffix ((trfirst mtr').2 !!! saB) (s.2 !!! saB)))
-    as H.
-  { assert (∃ mtr'', after n' mtr' = Some mtr'') as H.
-    { apply (infinite_trace_after' (S n')) in Hafter as [mtr'' [Hmtr'' _]].
-      simpl in *. by eauto. }
-    destruct H as [mtr'' Hmtr''].
-    eapply (retransmit_fair_trace_buffer_grows _ _ mtr'') in Hn'' as Hbs';
-      [|by eapply mtrace_valid_after|done].
-    rewrite /pred_at Hmtr''. by destruct mtr''. }
-  replace (S n') with (n' + 1) by lia.
-  rewrite pred_at_sum. rewrite /pred_at in H. rewrite /pred_at in Hn'.
-  destruct (after n' mtr') as [mtr''|] eqn:Heqn; [|done].
-  assert (mtrace_valid mtr'') as Hvalid'.
-  { eapply mtrace_valid_after; [done|]. by eapply mtrace_valid_after. }
-  destruct mtr''; [naive_solver|].
-  rewrite pred_at_S /pred_at. rewrite Hbs in H.
-  inversion Hn'.
-  assert (label_role ℓ = inl Brole) as Heq.
-  { destruct ℓ; try naive_solver. }
-  destruct ℓ; simpl in *; simplify_eq. destruct r; simpl in *; simplify_eq.
-  punfold Hvalid'. inversion Hvalid'. simplify_eq.
-  inversion H2.
-  + destruct s0 as [[]]. simplify_eq. simpl in *.
-    destruct H as [? H]. rewrite H in H5. apply app_eq_nil in H5. set_solver.
-  + destruct mtr''=> /=; simpl in *; simplify_eq; set_solver.
-Qed.
-
-(* A trace starting in the receive role has partially terminated for the Brole *)
-Lemma retransmit_fair_traces_terminate_aux mtr :
-  (trfirst mtr).1.1 = Received → retransmit_terminating_role (Brole) mtr.
-Proof.
-  intros Htrfirst.
-  exists 0. rewrite /pred_at=> /=.
-  destruct mtr as [[[]]|[[]] l mtr];
-    simpl in *; simplify_eq; rewrite /retransmit_live_roles;
-    set_solver.
-Qed.
-
-(* Any fair trace terminates on role B *)
-Lemma retransmit_fair_traces_terminate mtr :
-  (trfirst mtr).1.1 = Start → mtrace_valid mtr → mtrace_fair mtr →
-  retransmit_terminating_role (Brole) mtr.
-Proof.
-  intros ???.
-  assert (infinite_trace mtr ∨ ¬ infinite_trace mtr) as [Hafter|Hafter];
-    [by apply ExcludedMiddle| |]; last first.
-  { apply not_forall_exists_not in Hafter as [n Hafter].
-    destruct (after n mtr) eqn:Heqn; [by naive_solver|].
-    exists n. by left. }
-  assert (∃ n, pred_at mtr n (λ st _, st.1.1 = Received)) as [n Hn].
-  { by apply retransmit_fair_trace_eventually_Received. }
-  rewrite /pred_at in Hn.
-  assert (∃ mtr', after n mtr = Some mtr') as [mtr' Hmtr'].
-  { destruct (after n mtr) as [mtr'|]; [|done]. by exists mtr'. }
-  rewrite Hmtr' in Hn.
-  assert ((trfirst mtr').1.1 = Received); [by destruct mtr'|].
-  assert (retransmit_terminating_role (Brole) mtr') as [m Hterminates];
-    [by apply retransmit_fair_traces_terminate_aux|].
-  exists (m+n). by rewrite pred_at_sum' after_sum Hmtr'.
-Qed.
 
 (* TODO: This is likely not needed. *)
 Lemma retransmit_live_spec_holds s ρ α s' :
   retransmit_trans s (inl (ρ,α)) s' → ρ ∈ retransmit_live_roles s.
 Proof. inversion 1; set_solver. Qed.
+
+Definition send_filter msg : retransmit_state → option retransmit_label → Prop :=
+  λ _ l, option_map label_action l = Some $ inl $ Some msg.
+Instance send_filter_decision msg st l : Decision (send_filter msg st l).
+Proof. apply make_decision. Qed.
+
+Definition deliver_filter msg : retransmit_state → option retransmit_label → Prop :=
+  λ _ l, l = Some $ inr ((),Some msg).
+Instance deliver_filter_decision msg st l : Decision (deliver_filter msg st l).
+Proof. apply make_decision. Qed.
+
+Definition retransmit_fair_network_delivery msg : mtrace → Prop :=
+  □ (□◊↓send_filter msg → ◊↓deliver_filter msg).
+
+Definition retransmit_fair_network (mtr : mtrace) : Prop :=
+  ∀ msg, retransmit_fair_network_delivery msg mtr.
+
+(* TODO: This should be generalised, and lifted to multiple roles *)
+Definition retransmit_terminating_role (ρ : retransmit_node_role) (tr : mtrace) : Prop :=
+  (◊↓λ st _, ρ ∉ retransmit_live_roles st) tr ∨ ¬ infinite_trace tr.
+
+Definition retransmit_fair_scheduling_mtr (ρ : retransmit_node_role) : mtrace → Prop :=
+  trace_always_eventually_implies_now
+    (λ δ _, retransmit_role_enabled_model ρ δ)
+    (λ δ ℓ, ¬ retransmit_role_enabled_model ρ δ ∨
+              option_map label_role ℓ = Some (inl ρ)).
+
+Definition retransmit_fair_scheduling (mtr : mtrace) : Prop :=
+  ∀ ρ, retransmit_fair_scheduling_mtr ρ mtr.
+
+Definition mtrace_fair (mtr : mtrace) : Prop :=
+  retransmit_fair_scheduling mtr ∧ retransmit_fair_network mtr.
+
+Lemma mtrace_fair_always mtr :
+  mtrace_fair mtr ↔ (□ mtrace_fair) mtr.
+Proof. 
+  split.
+  - rewrite /mtrace_fair.
+    intros [Hmtr1 Hmtr2].
+    rewrite /retransmit_fair_scheduling in Hmtr1.
+    rewrite /retransmit_fair_network in Hmtr2.
+    rewrite /retransmit_fair_scheduling_mtr in Hmtr1.
+    rewrite /retransmit_fair_network_delivery in Hmtr2.
+    apply trace_always_forall in Hmtr1.
+    apply trace_always_forall in Hmtr2.
+    eassert ((□ trace_and _ _) mtr).
+    { apply trace_always_and. split; [apply Hmtr1|apply Hmtr2]. }
+    apply trace_always_idemp in H.
+    revert H. apply trace_always_mono.
+    intros tr.
+    apply trace_impliesI.
+    intros Htr.
+    apply trace_always_and in Htr as [Htr1 Htr2].
+    split.
+    + intros x. revert Htr1. 
+      apply trace_always_mono. intros tr'. apply trace_impliesI.
+      intros Htr'. done.
+    + intros x. revert Htr2. 
+      apply trace_always_mono. intros tr'. apply trace_impliesI.
+      intros Htr'. done.
+  - by intros Hfair%trace_always_elim.
+Qed.
+
+Definition trans_valid (mtr : mtrace) :=
+   match mtr with
+   | ⟨s⟩ => True
+   | (s -[l]-> tr) => retransmit_trans s l (trfirst tr)
+   end.
+
+Definition mtrace_valid (mtr : mtrace) :=
+  trace_always trans_valid mtr.
+
+Definition option_lift {S L} (P : S → L → Prop) : S → option L → Prop :=
+  λ s ol, ∃ l, ol = Some l ∧ P s l.
+
+Lemma option_lift_Some {S L} (P : S → L → Prop) s l :
+  option_lift P s (Some l) → P s l.
+Proof. intros (l'&Hl'&HP). by simplify_eq. Qed.
+
+Lemma A_always_live (mtr : mtrace) :
+  (□ (trace_now (λ s _, retransmit_role_enabled_model Arole s))) mtr.
+Proof. apply trace_always_universal.
+  rewrite /pred_at /retransmit_role_enabled_model. intros mtr'.
+  by destruct mtr'; set_solver.
+Qed.
+
+Lemma retransmit_fair_traces_eventually_A mtr :
+  retransmit_fair_scheduling_mtr Arole mtr →
+  (◊ (↓ (λ _ ℓ, option_map label_role ℓ = Some $ inl Arole))) mtr.
+Proof.
+  intros Hfair.
+  pose proof (A_always_live mtr) as HA.
+  eapply trace_always_eventually_always_implies; [|done].
+  eapply trace_always_eventually_always_mono; [| |apply Hfair].
+  - intros Htr. apply trace_implies_refl.
+  - intros tr.
+    apply trace_impliesI.
+    apply trace_now_mono.
+    intros s l. intros [Htr|Htr]; [|done].
+    rewrite /retransmit_role_enabled_model in Htr. set_solver.
+Qed.
+
+Lemma retransmit_fair_traces_eventually_mAB mtr :
+  mtrace_valid mtr → retransmit_fair_scheduling_mtr Arole mtr →
+  (◊ ↓ send_filter mAB) mtr.
+Proof.
+  intros Hvalid Hfair.
+  pose proof (retransmit_fair_traces_eventually_A mtr Hfair) as Htr.
+  eapply trace_eventually_mono_strong; [|done].
+  intros tr' Htr'.
+  eapply trace_always_suffix_of in Hvalid; [|done].
+  apply trace_always_elim in Hvalid.
+  destruct tr' as [s|s l tr']; [done|].
+  apply trace_now_mono_strong.
+  intros ???? HP; simplify_eq.
+  destruct l; [|done]. destruct r. simpl in *.
+  simplify_eq. inversion Hvalid. inversion H1. by simplify_eq.
+Qed.
+
+(* Proof by the fact that A is always live, and will eventually be scheduled.
+   Needs fairness assumptions *)
+Lemma retransmit_fair_traces_always_eventually_mAB mtr :
+  mtrace_valid mtr → retransmit_fair_scheduling_mtr Arole mtr →
+  (□ ◊ ↓ send_filter mAB) mtr.
+Proof.
+  intros Hvalid Hfair. eapply trace_always_implies_always;
+    [|apply trace_always_and; split; [apply Hvalid|apply Hfair]].
+  intros tr' [Hvalid' Hfair']%trace_always_and.
+  by apply retransmit_fair_traces_eventually_mAB.
+Qed.
+
+Lemma eventually_send_eventually_deliver mtr :
+  retransmit_fair_network mtr →
+  (□ ◊ ↓ send_filter mAB) mtr →
+  (◊ ↓ deliver_filter mAB) mtr.
+Proof.
+  intros Hfair_network Hsend.
+  pose proof (Hfair_network mAB). apply trace_always_elim in H.
+  rewrite trace_impliesI in H. apply H. done.
+Qed.
+
+(* If a message is delivered, the next state has a message in the buffer *)
+(* Proof by validity relation of the model *)
+Lemma deliver_next_buffer msg mtr :
+  mtrace_valid mtr →
+  (↓ deliver_filter msg) mtr →
+  (○ ↓ λ s _, ∃ bs, s.2 !!! (m_destination msg) = msg :: bs) mtr.
+Proof.
+  intros Hvalid%trace_always_elim Hdeliver.
+  destruct mtr; [done|].
+  exists mtr. split; [done|].
+  rewrite /trace_now /deliver_filter /pred_at in Hdeliver.
+  simpl in *. simplify_eq.
+  inversion Hvalid. simplify_eq.
+  destruct mtr.
+  - rewrite /trace_now /pred_at. simpl in *. simplify_eq.
+    exists (bs !!! m_destination msg).
+    simpl. by rewrite lookup_total_insert.
+  - rewrite /trace_now /pred_at. simpl in *. simplify_eq.
+    exists (bs !!! m_destination msg).
+    simpl. by rewrite lookup_total_insert.
+Qed.
+
+(* A scheduled B will succeed if there is something in the buffer *)
+(* Proof by validity relation of the model *)
+Lemma successful_deliver_received bs (mtr : mtrace) :
+  mtrace_valid mtr →
+  (↓ (λ s _, mAB :: bs `suffix_of` s.2 !!! (m_destination mAB))) mtr →
+  (↓ (λ _ l, option_map label_role l = Some (inl Brole))) mtr →
+  (○ ↓ (λ s _, s.1.1 = Received)) mtr.
+Proof.
+  intros Hvalid%trace_always_elim Hbs HB.
+  destruct mtr as [?|s l mtr]; [done|].
+  simpl in *. destruct l as [|]; [|done].
+  exists mtr. split; [done|].
+  rewrite /trace_now /pred_at in HB.
+  simpl in *. simplify_eq.
+  destruct r. simpl in *. simplify_eq.
+  inversion Hvalid; simplify_eq; [|]; last first.
+  { destruct mtr as [[]|[]]; simpl in *; simplify_eq; done. }
+    rewrite /trace_now /pred_at in Hbs. simpl in *.
+  rewrite H2 in Hbs. by apply suffix_cons_nil_inv in Hbs.
+Qed.
+
+Lemma B_enabled_not_received s :
+  retransmit_role_enabled_model Brole s ↔ s.1.1 ≠ Received.
+Proof.
+  rewrite /retransmit_role_enabled_model /retransmit_live_roles.
+  split.
+  - intros. destruct s as [[??]?]. simpl in *. intros ->. set_solver.
+  - intros. destruct s as [[??]?]. simpl in *.
+    apply elem_of_union. right. destruct r; set_solver.
+Qed.
+
+Lemma not_B_enabled_received s :
+  ¬ retransmit_role_enabled_model Brole s ↔ s.1.1 = Received.
+Proof.
+  rewrite /retransmit_role_enabled_model /retransmit_live_roles.
+  split.
+  - intros. destruct s as [[??]?]. simpl in *. destruct r; set_solver.
+  - intros. destruct s as [[??]?]. simpl in *. intros Helem.
+    simplify_eq. set_solver.
+Qed.
+
+Lemma received_or_eventually_B (mtr : mtrace) :
+  mtrace_fair mtr →
+  (◊↓ λ s _, s.1.1 = Received) mtr ∨
+  (◊↓ λ _ l, option_map label_role l = Some $ inl Brole) mtr.
+Proof.
+  intros Hfair.
+  assert ((↓ λ s _, s.1.1 = Received) mtr ∨
+         ¬ (↓ λ s _, s.1.1 = Received) mtr).
+  { apply ExcludedMiddle. }
+  destruct H as [H|H].
+  { left. apply trace_eventually_intro. done. }
+  apply trace_notI in H. apply trace_now_not in H.
+  assert ((↓ (λ s _, retransmit_role_enabled_model Brole s)) mtr) as HB.
+  { revert H. apply trace_now_mono.
+    intros. by apply B_enabled_not_received. }
+  destruct Hfair as [Hfair _].
+  specialize (Hfair Brole).
+  apply trace_always_elim in Hfair.
+  rewrite trace_impliesI in Hfair.
+  apply Hfair in HB.
+  apply trace_eventually_or. revert HB.
+  apply trace_eventually_mono.
+  intros tr Htr.
+  apply trace_now_or in Htr.
+  destruct Htr as [Htr|Htr].
+  - left. revert Htr. apply trace_now_mono. intros.
+    by apply not_B_enabled_received.
+  - by right.
+Qed.
+
+(* Need to assume that trace is infinite *)
+Lemma retransmit_fair_trace_buffer_grow_next mtr bs :
+  infinite_trace mtr →
+  mtrace_valid mtr →
+  (↓ λ s _, s.2 !!! (m_destination mAB) = bs) mtr →
+  (↓ λ _ l, option_map label_role l ≠ Some $ inl Brole) mtr →
+  (○ (↓ (λ s _, ∃ bs', bs `suffix_of` bs' ∧
+                       s.2 !!! m_destination mAB = bs'))) mtr.
+Proof.
+  intros Hinf Hvalid Hbs HBrole.
+  apply trace_always_elim in Hvalid.
+  destruct mtr.
+  { specialize (Hinf 1). by apply is_Some_None in Hinf. }
+  destruct mtr.
+  { specialize (Hinf 2). by apply is_Some_None in Hinf. }
+  destruct s as [[??]?].
+  rewrite /trace_now /pred_at.
+  rewrite /trace_now /pred_at in Hbs.
+  rewrite /trace_now /pred_at in HBrole.
+  simpl in *.
+  apply trace_next_intro.
+  inversion Hvalid; simplify_eq.
+  - exists (g !!! m_destination mAB). set_solver.
+  - exists (g !!! m_destination mAB). set_solver.
+  - exists (g !!! m_destination mAB). set_solver.
+  - destruct (decide (m_destination msg = saB)) as [->|Hneq].
+    + exists (msg :: g !!! m_destination mAB).
+      split; [by apply suffix_cons_r|].
+      simpl. rewrite lookup_total_insert. done.
+    + exists (g !!! m_destination mAB).
+      simpl. rewrite lookup_total_insert_ne; [|done].
+      set_solver.
+Qed.
+
+(* The buffers will only grow until B is scheduled *)
+(* Proof by validity relation of the model *)
+Lemma retransmit_fair_trace_buffer_grows mtr bs :
+  infinite_trace mtr →
+  mtrace_valid mtr →
+  mtrace_fair mtr →
+  (↓ λ s _, s.2 !!! (m_destination mAB) = bs) mtr →
+  ((◊trace_and
+     (↓ (λ s _, suffix bs (s.2 !!! (m_destination mAB))))
+     (↓ (λ _ l, option_map label_role l = Some $ inl Brole))) mtr) ∨
+  ((◊↓ λ s _, s.1.1 = Received) mtr).
+Proof.
+  intros Hinf Hvalid Hfair Hnow.
+  (* TODO: Need to assume not received instead *)
+  pose proof (received_or_eventually_B mtr Hfair) as [Hreceived|HB].
+  { right. done. }
+  left.
+  revert bs Hnow.
+  apply trace_eventually_until in HB.
+  induction HB; intros bs Hnow.
+  { eapply trace_eventually_mono; [apply trace_now_and|].
+    apply trace_eventually_intro.
+    pose proof (trace_now_split _ _ _ Hnow H) as Hnow'.
+    revert Hnow'. apply trace_now_mono.
+    intros s l [H1 H2]. split; [|done]. set_solver. }
+  apply trace_eventually_cons.
+  assert (∃ bs', bs `suffix_of` bs' ∧
+             (↓ (λ s _ , s.2 !!! m_destination mAB = bs'))
+               tr) as [bs' [Hbs' Hnow']].
+  { assert ((↓ (λ s _, ∃ bs', bs `suffix_of` bs' ∧ s.2 !!! m_destination mAB = bs'))
+               tr) as H'; last first.
+    { apply trace_now_exists in H' as [bs' H'].
+      exists bs'.
+      rewrite /trace_now /pred_at.
+      rewrite /trace_now /pred_at in H'.
+      destruct tr; simpl in *; done. }
+    eapply trace_next_elim.
+    by apply retransmit_fair_trace_buffer_grow_next. }
+    eapply trace_eventually_mono; last first.
+  { assert (mtrace_valid tr) as Hvalid' by by eapply trace_always_cons.
+    apply mtrace_fair_always in Hfair.
+    assert (mtrace_fair tr) as Hfair'.
+    { apply mtrace_fair_always. by eapply trace_always_cons. }
+    assert (infinite_trace tr) as Hinf'.
+    { by eapply infinite_cons. }
+    apply (IHHB Hinf' Hvalid' Hfair' bs').
+    done. }
+  intros tr' H'. apply trace_andI. apply trace_andI in H'.
+  destruct H' as [H1 H2].
+  split; [|done].
+  revert H1. apply trace_now_mono.
+  intros ???. by etransitivity.
+Qed.
+
+Lemma eventually_deliver_eventually_received mtr :
+  infinite_trace mtr → mtrace_valid mtr → mtrace_fair mtr →
+  (◊ ↓ deliver_filter mAB) mtr →
+  (◊ ↓ λ s _, s.1.1 = Received) mtr.
+Proof.
+  intros Hinf Hvalid Hfair Hdeliver.
+  eapply trace_eventually_mono_strong in Hdeliver; last first.
+  { intros tr' Hsuffix. apply deliver_next_buffer. by eapply trace_always_suffix_of. }
+  apply trace_eventually_next in Hdeliver.
+  apply trace_eventually_idemp.
+  revert Hdeliver.
+  apply trace_eventually_mono_strong.
+  intros mtr' Hsuffix Hdeliver.
+  apply trace_now_exists in Hdeliver as [bs Hdeliver].
+  assert (infinite_trace mtr') as Hinf'.
+  { destruct Hsuffix as [n Hn].
+    eapply (infinite_trace_after n) in Hinf.
+    by rewrite Hn in Hinf. }
+  assert (mtrace_valid mtr') as Hvalid'.
+  { by eapply trace_always_suffix_of. }
+  assert (mtrace_fair mtr') as Hfair'.
+  { apply mtrace_fair_always in Hfair.
+    apply mtrace_fair_always. by eapply trace_always_suffix_of. }
+  pose proof (retransmit_fair_trace_buffer_grows _ (mAB :: bs) Hinf' Hvalid' Hfair' Hdeliver) as [H'|H']; last first.
+  { done. }
+  apply trace_eventually_next.
+  revert H'.
+  apply trace_eventually_mono_strong.
+  intros mtr'' Hsuffix' [Hmtr1'' Hmtr2'']%trace_andI.
+  assert (mtrace_valid mtr'') by by eapply trace_always_suffix_of.
+  by eapply successful_deliver_received.
+Qed.
+
+(* Any fair trace terminates on role B *)
+Lemma retransmit_fair_traces_terminate mtr :
+  mtrace_valid mtr → mtrace_fair mtr →
+  retransmit_terminating_role Brole mtr.
+Proof.
+  intros Hvalid [Hfair1 Hfair2].
+  assert (infinite_trace mtr ∨ ¬ infinite_trace mtr) as [Hafter|Hafter];
+    [by apply ExcludedMiddle| |]; last first.
+  { by right. }
+  left.
+  pose proof (retransmit_fair_traces_always_eventually_mAB mtr Hvalid (Hfair1 _)).
+  apply (eventually_send_eventually_deliver _ Hfair2) in H.
+  apply (eventually_deliver_eventually_received) in H; [|done..].
+  revert H. apply trace_eventually_mono.
+  intros tr. apply trace_now_mono. intros [[]] _ Hreceived.
+  rewrite /retransmit_live_roles. simpl in *.
+  simplify_eq. set_solver.
+Qed.
 
 Definition retransmit_fair_model : FairModel.
 Proof.
@@ -483,7 +522,7 @@ Proof.
             fmaction := retransmit_node_action;
             fmconfig := retransmit_network_label;
             fmtrans := retransmit_trans;
-            fmfairness := retransmit_network_fair_delivery;
+            fmfairness := retransmit_fair_network;
             live_roles := retransmit_live_roles;
             fm_live_spec := retransmit_live_spec_holds;
           |}).
